tools/Vale/src/emit_fstar_text.fs
@@ -172,9 +172,10 @@ let rec emit_stmt (ps:print_state) (outs:formal list option) (s:stmt):unit =
   | SAssume e -> ps.PrintLine ("assume " + (string_of_exp e) + ";")
   | SAssert (_, e) -> ps.PrintLine ("assert " + (string_of_exp e) + ";")
   | SCalc _ -> err "unsupported feature: 'calc' for F*"
-  | SVar (x, tOpt, _, g, a, eOpt) ->
+  | SVar (x, tOpt, _, g, a, None) -> () // used to forward-declare variables for SLetUpdates
+  | SVar (x, tOpt, _, g, a, Some e) ->
       let sf = string_of_formal (x, tOpt) in
-      let rhs = match eOpt with Some e -> " = " + (string_of_exp e) | None -> err "right-hand side required in variable declaration" in
+      let rhs = " = " + (string_of_exp e) in
       ps.PrintLine ((string_of_var_storage g) + "let " + sf + rhs + " in")
   | SAlias _ -> internalErr "SAlias"
   | SAssign ([], e) -> ps.PrintLine ((string_of_exp e) + ";")
