src/arch/x64/X64.Vale.Lemmas_i.fst
@@ -4,9 +4,46 @@ open X64.Vale.State_i
 open FStar.UInt
 module S = X64.Semantics_s
 
-#reset-options "--initial_fuel 2 --max_fuel 2"
+#reset-options "--initial_fuel 2 --max_fuel 2 --z3rlimit 20"
 
-let eval_while b c n s0 s1 : Type0 = admit ()
+val increase_fuel (c:code) (s0:state) (f0:fuel) (sN:state) (fN:fuel) : Lemma
+  (requires eval_code c s0 f0 sN /\ f0 <= fN)
+  (ensures eval_code c s0 fN sN)
+  (decreases %[f0; c])
+
+val increase_fuels (c:codes) (s0:state) (f0:fuel) (sN:state) (fN:fuel) : Lemma
+  (requires eval_code (Block c) s0 f0 sN /\ f0 <= fN)
+  (ensures eval_code (Block c) s0 fN sN)
+  (decreases %[f0; c])
+
+let rec increase_fuel (c:code) (s0:state) (f0:fuel) (sN:state) (fN:fuel) =
+  match c with
+  | Ins ins -> ()
+  | Block l -> increase_fuels l s0 f0 sN fN
+  | IfElse b t f ->
+      if eval_ocmp s0 b then increase_fuel t s0 f0 sN fN else increase_fuel f s0 f0 sN fN
+  | While b c ->
+      if not (eval_ocmp s0 b) then ()
+      else
+      (
+        match S.eval_code c (f0 - 1) (state_to_S s0) with
+        | None -> ()
+        | Some s1 ->
+            let s1 = state_of_S s1 in
+            increase_fuel c s0 (f0 - 1) s1 (fN - 1);
+            if s1.ok then increase_fuel (While b c) s1 (f0 - 1) sN (fN - 1)
+            else ()
+      )
+and increase_fuels (c:codes) (s0:state) (f0:fuel) (sN:state) (fN:fuel) =
+  match c with
+  | [] -> ()
+  | h::t ->
+    (
+      let Some s1 = S.eval_code h f0 (state_to_S s0) in
+      let s1 = state_of_S s1 in
+      increase_fuel h s0 f0 s1 fN;
+      increase_fuels t s1 f0 sN fN
+    )
 
 let lemma_cmp_eq s o1 o2 = ()
 let lemma_cmp_ne s o1 o2 = ()
@@ -15,22 +52,59 @@ let lemma_cmp_ge s o1 o2 = ()
 let lemma_cmp_lt s o1 o2 = ()
 let lemma_cmp_gt s o1 o2 = ()
 
-let lemma_block (b0:codes) (s0:state) (sN:state) =
-  let c1::b1 = b0 in
-  let s0' = state_to_S s0 in
-  // let Some s1' = S.eval_code c1 fuel s0' in
-  // let s1 = state_of_S s1' in
-  // (s1, c1, b1)
-  admit () // TODO
+let lemma_merge_total (b0:codes) (s0:state) (f0:fuel) (sM:state) (fM:fuel) (sN:state) =
+  let f = if f0 > fM then f0 else fM in
+  increase_fuel (Cons?.hd b0) s0 f0 sM f;
+  increase_fuel (Block (Cons?.tl b0)) sM fM sN f;
+  f
 
-let lemma_empty (s0:state) (sN:state) =
-  assume False; // TODO
-  s0
+let lemma_empty_total (s0:state) (bN:codes) =
+  (s0, 0)
 
-let lemma_ifElse (ifb:S.ocmp) (ct:code) (cf:code) (s0:state) (sN:state) =
-  (eval_ocmp s0 ifb, s0)
+let lemma_ifElse_total (ifb:ocmp) (ct:code) (cf:code) (s0:state) =
+  (eval_ocmp s0 ifb, s0, s0, 0)
 
-let lemma_while b c s0 sN = admit () // TODO
-let lemma_whileTrue b c n s0 sN = admit () // TODO
-let lemma_whileFalse b c s0 sN = admit () // TODO
+let lemma_ifElseTrue_total (ifb:ocmp) (ct:code) (cf:code) (s0:state) (f0:fuel) (sM:state) =
+  ()
 
+let lemma_ifElseFalse_total (ifb:ocmp) (ct:code) (cf:code) (s0:state) (f0:fuel) (sM:state) =
+  ()
+
+let eval_while_inv_temp (c:code) (s0:state) (fW:fuel) (sW:state) : Type0 =
+  forall (f:nat).{:pattern S.eval_code c f (state_to_S sW)}
+    Some? (S.eval_code c f (state_to_S sW)) ==>
+    S.eval_code c (f + fW) (state_to_S s0) == S.eval_code c f (state_to_S sW)
+
+let eval_while_inv (c:code) (s0:state) (fW:fuel) (sW:state) : Type0 =
+  eval_while_inv_temp c s0 fW sW
+
+let lemma_while_total (b:ocmp) (c:code) (s0:state) =
+  (s0, 0)
+
+let lemma_whileTrue_total (b:ocmp) (c:code) (s0:state) (sW:state) (fW:fuel) =
+  (sW, fW)
+
+let lemma_whileFalse_total (b:ocmp) (c:code) (s0:state) (sW:state) (fW:fuel) =
+  let f1 = fW + 1 in
+  assert (S.eval_code (While b c) f1 (state_to_S s0) == S.eval_code (While b c) 1 (state_to_S sW));
+  assert (eval_code (While b c) s0 f1 sW);
+  (sW, f1)
+
+let lemma_whileMerge_total (c:code) (s0:state) (f0:fuel) (sM:state) (fM:fuel) (sN:state) =
+  let fN:nat = f0 + fM + 1 in
+  let fForall (f:nat) : Lemma
+    (requires Some? (S.eval_code c f (state_to_S sN)))
+    (ensures S.eval_code c (f + fN) (state_to_S s0) == S.eval_code c f (state_to_S sN)) =
+    let Some sZ = S.eval_code c f (state_to_S sN) in
+    let fZ = if f > fM then f else fM in
+    increase_fuel (While?.whileBody c) sM fM sN fZ;
+    increase_fuel c sN f (state_of_S sZ) fZ;
+    assert (S.eval_code c (fZ + 1) (state_to_S sM) == Some sZ);
+    assert (S.eval_code c (fZ + 1) (state_to_S sM) == S.eval_code c (fZ + 1 + f0) (state_to_S s0));
+    assert (S.eval_code c (fZ + 1 + f0) (state_to_S s0) == Some sZ);
+    increase_fuel c s0 (fZ + 1 + f0) (state_of_S sZ) (f + fN);
+    assert (S.eval_code c (f + fN) (state_to_S s0) == Some sZ);
+    ()
+    in
+  Classical.ghost_lemma fForall;
+  fN
